wip regalloc checker that iterates to compute loop invariant
(even though probably it only requires two iterations)

compiler/src/compiler/RegAlloc4.v
@@ -15,6 +15,7 @@ Require Import coqutil.Map.TestLemmas.
 Require Import bedrock2.Syntax.
 Require Import coqutil.Datatypes.ListSet.
 Require Import coqutil.Tactics.Simp.
+Require Import coqutil.Tactics.autoforward.
 Require Import compiler.Simulation.
 
 Open Scope Z_scope.
@@ -25,6 +26,8 @@ Local Notation stmt  := (@FlatImp.stmt srcvar). (* input type *)
 Local Notation stmt' := (@FlatImp.stmt impvar). (* output type *)
 Local Notation bcond  := (@FlatImp.bcond srcvar).
 Local Notation bcond' := (@FlatImp.bcond impvar).
+
+Axiom TODO_sam: False.
 
 Definition accessed_vars_bcond(c: bcond): list srcvar :=
   match c with
@@ -59,12 +62,12 @@ https://github.com/mit-plv/bedrock2/tree/7cbae1a1caf7d19270d0fb37199f86eb8ea5ce4
 
 Declare Scope option_monad_scope. Local Open Scope option_monad_scope.
 
-Notation "c1 ;; c2" :=
+Notation "' pat <- c1 ;; c2" :=
   (match c1 with
-   | Some _ => c2
+   | Some pat => c2
    | None => None
    end)
-  (at level 61, right associativity) : option_monad_scope.
+  (at level 61, pat pattern, c1 at next level, right associativity) : option_monad_scope.
 
 Notation "x <- c1 ;; c2" :=
   (match c1 with
@@ -73,12 +76,12 @@ Notation "x <- c1 ;; c2" :=
    end)
   (at level 61, c1 at next level, right associativity) : option_monad_scope.
 
-Notation "' pat <- c1 ;; c2" :=
+Notation "c1 ;; c2" :=
   (match c1 with
-   | Some pat => c2
+   | Some _ => c2
    | None => None
    end)
-  (at level 61, pat pattern, c1 at next level, right associativity) : option_monad_scope.
+  (at level 61, right associativity) : option_monad_scope.
 
 Scheme Equality for Syntax.access_size. (* to create access_size_beq *)
 Scheme Equality for bopname. (* to create bopname_beq *)
@@ -95,84 +98,511 @@ Module Byte.
   Qed.
 End Byte.
 
-Module map.
-  Class ops{K V: Type}(M: map.map K V) := {
-    intersect: M -> M -> M; (* set intersection when interpreting maps as sets of tuples *)
-  }.
-End map.
+Section PairList.
+  Context {A B: Type}.
+
+  Definition remove_by_fst(aeqb: A -> A -> bool)(key: A): list (A * B) -> list (A * B) :=
+    List.filter (fun '(a, b) => negb (aeqb a key)).
+
+  Definition remove_by_snd(beqb: B -> B -> bool)(key: B): list (A * B) -> list (A * B) :=
+    List.filter (fun '(a, b) => negb (beqb b key)).
+
+  Lemma In_remove_by_fst{aeqb: A -> A -> bool}{aeqb_spec: EqDecider aeqb}: forall a a' b l,
+      In (a, b) (remove_by_fst aeqb a' l) ->
+      In (a, b) l /\ a <> a'.
+  Proof.
+    unfold remove_by_fst. intros. eapply filter_In in H. destruct H.
+    destr (aeqb a a'). 1: discriminate. auto.
+  Qed.
+
+  Lemma not_In_remove_by_snd{beqb: B -> B -> bool}{beqb_spec: EqDecider beqb}: forall a b l,
+      ~ In (a, b) (remove_by_snd beqb b l).
+  Proof.
+    unfold remove_by_snd, not. intros. eapply filter_In in H. apply proj2 in H.
+    destr (beqb b b). 1: discriminate. apply E. reflexivity.
+  Qed.
+
+  Lemma In_remove_by_snd{beqb: B -> B -> bool}{beqb_spec: EqDecider beqb}: forall a b b' l,
+      In (a, b) (remove_by_snd beqb b' l) ->
+      In (a, b) l /\ b <> b'.
+  Proof.
+    unfold remove_by_snd. intros. eapply filter_In in H. destruct H.
+    destr (beqb b b'). 1: discriminate. auto.
+  Qed.
+End PairList.
+
+Section IntersectLemmas.
+  Context {A: Type}(aeqb: A -> A -> bool){aeqb_spec: EqDecider aeqb}.
+
+  Lemma intersect_max_length_l: forall l1 l2,
+      (length (list_intersect aeqb l1 l2) <= length l1)%nat.
+  Proof.
+    intros.
+    induction l1; intros.
+    - simpl. reflexivity.
+    - unfold list_intersect in *. cbn [fold_right]. destruct_one_match.
+      + cbn [length]. eapply Peano.le_n_S. apply IHl1.
+      + cbn [length]. eapply Nat.le_trans. 1: apply IHl1. constructor. reflexivity.
+  Qed.
+
+  Lemma intersect_same_length: forall l1 l2,
+      length (list_intersect aeqb l1 l2) = length l1 ->
+      list_intersect aeqb l1 l2 = l1.
+  Proof.
+    induction l1; intros.
+    - reflexivity.
+    - simpl in *. destruct_one_match; simpl in *.
+      + f_equal. eapply IHl1. congruence.
+      + pose proof (intersect_max_length_l l1 l2) as P.
+        rewrite H in P. exfalso. eapply Nat.nle_succ_diag_l. exact P.
+  Qed.
+End IntersectLemmas.
 
 #[export] Hint Resolve Byte.eqb_spec : typeclass_instances.
 
 Definition assert(b: bool): option unit := if b then Some tt else None.
 
-Section RegAlloc.
+Definition mapping_eqb: srcvar * impvar -> srcvar * impvar -> bool :=
+  fun '(x, x') '(y, y') => andb (String.eqb x y) (Z.eqb x' y').
 
-  Context {src2imp: map.map srcvar impvar}.
-  Context {src2impOk: map.ok src2imp}.
-  Context {imp2src: map.map impvar srcvar} {imp2srcOps: map.ops imp2src}.
-  Context {imp2srcOk: map.ok imp2src}.
+Definition assert_in(y: srcvar)(y': impvar)(m: list (srcvar * impvar)): option unit :=
+  _ <- List.find (mapping_eqb (y, y')) m;; Some tt.
 
-  (* "bindings" from impvar to srcvar that hold for sure after executing s:
-     Q: how to implement loop case? Does it have to iterate until a fixpoint is reached?
-
-     What if we just return those of s1?
-
-     But if we chain it on top of a previous bindings, and s2 gets executed, that might invalidate some
-     bindings --> need the concept of "update := add|remove" ??
-
-     *)
-  Definition assert_maps(m: imp2src)(y': impvar)(y: srcvar): option unit :=
-    y0 <- map.get m y';; assert (String.eqb y0 y).
-
-  Definition check_bcond(m: imp2src)(c: bcond)(c': bcond'): option unit :=
-    match c, c' with
-    | CondBinary op y z, CondBinary op' y' z' =>
-      assert_maps m y' y;; assert_maps m z' z;; assert (bbinop_beq op op')
-    | CondNez y, CondNez y' =>
-      assert_maps m y' y
-    | _, _ => None
+Definition check_bcond(m: list (srcvar * impvar))(c: bcond)(c': bcond'): option unit :=
+  match c, c' with
+  | CondBinary op y z, CondBinary op' y' z' =>
+    assert_in y y' m;; assert_in z z' m;; assert (bbinop_beq op op')
+  | CondNez y, CondNez y' =>
+    assert_in y y' m
+  | _, _ => None
   end.
 
-  (* does 2 things at once: checks that the correct variables are read and computes the bindings
-     that hold after executing the statement *)
-  (* m: conservative underapproximation of which impvar stores which srcvar *)
-  Fixpoint check(m: imp2src)(s: stmt)(s': stmt'){struct s}: option imp2src :=
-    match s, s' with
-    | SSet x y, SSet x' y' =>
-      assert_maps m y' y;; Some (map.put m x' x)
-    | SLoad sz x y ofs, SLoad sz' x' y' ofs' =>
-      assert_maps m y' y;;
-      assert (Z.eqb ofs ofs');;
-      assert (access_size_beq sz sz');;
-      Some (map.put m x' x)
-    | SInlinetable sz x bs y, SInlinetable sz' x' bs' y' =>
-      assert_maps m y' y;;
-      assert (access_size_beq sz sz');;
-      assert (List.list_eqb Byte.eqb bs bs');;
-      Some (map.put m x' x)
-    | SLit x z, SLit x' z' =>
-      assert (Z.eqb z z');;
-      Some (map.put m x' x)
-    | SOp x op y z, SOp x' op' y' z' =>
-      assert_maps m y' y;;
-      assert_maps m z' z;;
-      assert (bopname_beq op op');;
-      Some (map.put m x' x)
-    | SIf c s1 s2, SIf c' s1' s2' =>
-      check_bcond m c c';;
+Definition assignment(m: list (srcvar * impvar))(x: srcvar)(x': impvar): list (srcvar * impvar) :=
+  (x, x') :: (remove_by_snd Z.eqb x' (remove_by_fst String.eqb x m)).
+
+Section LoopInv.
+  Context (check: list (srcvar * impvar) -> stmt -> stmt' -> option (list (srcvar * impvar)))
+          (s1 s2: stmt)(s1' s2': stmt').
+
+  (* Probably one iteration to compute the invariant, and another one to check that it
+     doesn't change any more, ie 2 iterations, is enough, but that might be hard to prove.
+     `List.length m` is enough fuel because the size can decrease at most that many times
+     before we get to an empty invariant. *)
+  Fixpoint loop_inv'(fuel: nat)(m: list (srcvar * impvar)): option (list (srcvar * impvar)) :=
+    match fuel with
+    | O => None
+    | S fuel' =>
       m1 <- check m s1 s1';;
-      m2 <- check m s2 s2';;
-      Some (map.intersect m1 m2)
-    | SSeq s1 s2, SSeq s1' s2' =>
-      m1 <- check m s1 s1';;
-      check m1 s2 s2'
-    | SLoop s1 c s2, SLoop s1' c' s2' =>
-      m1 <- check m s1 s1';;
-      check_bcond m1 c c';;
       m2 <- check m1 s2 s2';;
-      (* need to check again because next loop iteration is done with m2 instead of m!! *)
-      None
-    | _, _ => None
+      let cand := list_intersect mapping_eqb m m2 in
+      if Nat.eqb (List.length m) (List.length cand)
+      then Some cand
+      else loop_inv' fuel' cand
+    end.
+End LoopInv.
+
+(* does 2 things at once: checks that the correct variables are read and computes the bindings
+   that hold after executing the statement *)
+(* m: conservative underapproximation of which impvar stores which srcvar *)
+Fixpoint check(m: list (srcvar * impvar))(s: stmt)(s': stmt'){struct s}: option (list (srcvar * impvar)) :=
+  match s, s' with
+  | SLoad sz x y ofs, SLoad sz' x' y' ofs' =>
+    assert_in y y' m;;
+    assert (Z.eqb ofs ofs');;
+    assert (access_size_beq sz sz');;
+    Some (assignment m x x')
+  | SStore sz x y ofs, SStore sz' x' y' ofs' =>
+    assert_in x x' m;;
+    assert_in y y' m;;
+    assert (Z.eqb ofs ofs');;
+    assert (access_size_beq sz sz');;
+    Some m
+  | SInlinetable sz x bs y, SInlinetable sz' x' bs' y' =>
+    assert_in y y' m;;
+    assert (access_size_beq sz sz');;
+    assert (List.list_eqb Byte.eqb bs bs');;
+    Some (assignment m x x')
+  | SStackalloc x n body, SStackalloc x' n' body' =>
+    None (* TODO *)
+  | SLit x z, SLit x' z' =>
+    assert (Z.eqb z z');;
+    Some (assignment m x x')
+  | SOp x op y z, SOp x' op' y' z' =>
+    assert_in y y' m;;
+    assert_in z z' m;;
+    assert (bopname_beq op op');;
+    Some (assignment m x x')
+  | SSet x y, SSet x' y' =>
+    assert_in y y' m;; Some (assignment m x x')
+  | SIf c s1 s2, SIf c' s1' s2' =>
+    check_bcond m c c';;
+    m1 <- check m s1 s1';;
+    m2 <- check m s2 s2';;
+    Some (list_intersect mapping_eqb m1 m2)
+  | SLoop s1 c s2, SLoop s1' c' s2' =>
+    inv <- loop_inv' check s1 s2 s1' s2' (List.length m) m;;
+    m1 <- check inv s1 s1';;
+    check_bcond m1 c c';;
+    m2 <- check m1 s2 s2';;
+    Some m1
+  | SSeq s1 s2, SSeq s1' s2' =>
+    m1 <- check m s1 s1';;
+    check m1 s2 s2'
+  | SSkip, SSkip =>
+    Some m
+  | SCall binds f args, SCall binds' f' args' =>
+    None (* TODO *)
+  | SInteract binds f args, SInteract binds' f' args' =>
+    None (* TODO *)
+  | _, _ => None
+  end.
+
+Definition loop_inv(corresp: list (srcvar * impvar))(s1 s2: stmt)(s1' s2': stmt'): list (srcvar * impvar) :=
+  match loop_inv' check s1 s2 s1' s2' (List.length corresp) corresp with
+  | Some inv => inv
+  | None => []
+  end.
+
+Definition extends(m1 m2: list (srcvar * impvar)): Prop :=
+  forall x x', assert_in x x' m2 = Some tt -> assert_in x x' m1 = Some tt.
+
+Lemma extends_refl: forall m, extends m m.
+Proof. unfold extends. eauto. Qed.
+
+Lemma extends_nil: forall m, extends m [].
+Proof. unfold extends, assert_in. simpl. intros. discriminate. Qed.
+
+Lemma extends_trans: forall m1 m2 m3, extends m1 m2 -> extends m2 m3 -> extends m1 m3.
+Proof. unfold extends. eauto. Qed.
+
+Lemma extends_cons: forall a l1 l2,
+    extends l1 l2 ->
+    extends (a :: l1) (a :: l2).
+Proof.
+  unfold extends, assert_in. simpl. intros. simp.
+  destruct_one_match_hyp. 1: reflexivity.
+  eapply H. rewrite E. reflexivity.
+Qed.
+
+Lemma extends_cons_l: forall a l,
+    extends (a :: l) l.
+Proof.
+  unfold extends, assert_in. simpl. intros. simp.
+  destruct_one_match. 1: reflexivity.
+  destruct_one_match_hyp; discriminate.
+Qed.
+
+Lemma extends_cons_r: forall a l1 l2,
+    In a l1 ->
+    extends l1 l2 ->
+    extends l1 (a :: l2).
+Proof.
+  unfold extends, assert_in. simpl. intros. simp.
+  destruct_one_match_hyp. 2: {
+    eapply H0. rewrite E. reflexivity.
+  }
+  destruct_one_match. 1: reflexivity.
+  eapply find_none in E1. 2: eassumption.
+  simpl in E1. exfalso. congruence.
+Qed.
+
+Lemma extends_intersect_l: forall l1 l2,
+    extends l1 (list_intersect mapping_eqb l1 l2).
+Proof.
+  intros. induction l1; simpl.
+  - apply extends_refl.
+  - destruct_one_match.
+    + eapply extends_cons. apply IHl1.
+    + eapply extends_trans. 2: apply IHl1. apply extends_cons_l.
+Qed.
+
+Lemma extends_intersect_r: forall l1 l2,
+    extends l2 (list_intersect mapping_eqb l1 l2).
+Proof.
+  induction l1; intros.
+  - simpl. apply extends_nil.
+  - simpl. unfold mapping_eqb. destruct a as [x x']. destruct_one_match.
+    + destruct p as [z z']. eapply find_some in E. destruct E as [E1 E2].
+      apply Bool.andb_true_iff in E2. destruct E2 as [E2 E3].
+      autoforward with typeclass_instances in E2.
+      autoforward with typeclass_instances in E3.
+      subst z z'.
+      eapply extends_cons_r. 1: assumption. apply IHl1.
+    + apply IHl1.
+Qed.
+
+Lemma extends_loop_inv': forall s1 s2 s1' s2' fuel corresp1 corresp2,
+    loop_inv' check s1 s2 s1' s2' fuel corresp1 = Some corresp2 ->
+    extends corresp1 corresp2.
+Proof.
+  induction fuel; simpl; intros.
+  - discriminate.
+  - simp. destruct_one_match_hyp.
+    + simp. symmetry in E1. eapply intersect_same_length in E1.
+      rewrite E1. eapply extends_refl.
+    + eapply IHfuel in H. eapply extends_trans.
+      2: exact H. apply extends_intersect_l.
+Qed.
+
+Lemma extends_loop_inv: forall corresp s1 s2 s1' s2',
+    extends corresp (loop_inv corresp s1 s2 s1' s2').
+Proof.
+  intros. unfold loop_inv. destruct_one_match. 2: {
+    unfold extends. unfold assert_in. simpl. intros. discriminate.
+  }
+  eapply extends_loop_inv'. eassumption.
+Qed.
+
+Lemma defuel_loop_inv': forall fuel corresp inv m1 m2 s1 s2 s1' s2',
+    loop_inv' check s1 s2 s1' s2' fuel corresp = Some inv ->
+    check inv s1 s1' = Some m1 ->
+    check m1 s2 s2' = Some m2 ->
+    inv = list_intersect mapping_eqb inv m2.
+Proof.
+  induction fuel; intros; simpl in *.
+  - discriminate.
+  - simp. destruct_one_match_hyp.
+    + simp. symmetry in E1. eapply intersect_same_length in E1. rewrite E1 in H0.
+      rewrite E in H0. simp.
+      rewrite E0 in H1. simp.
+      rewrite <- E1 at 1. reflexivity.
+    + eapply IHfuel; eassumption.
+Qed.
+
+(* Similar effect as unfolding loop_inv where loop_inv's definition does not involve fuel,
+   ie this lemma allows us to prove `inv = intersect inv (update inv loop_body)` *)
+Lemma defuel_loop_inv: forall corresp inv m1 m2 s1 s2 s1' s2',
+    inv = loop_inv corresp s1 s2 s1' s2' ->
+    check inv s1 s1' = Some m1 ->
+    check m1 s2 s2' = Some m2 ->
+    inv = list_intersect mapping_eqb inv m2.
+Proof.
+  unfold loop_inv. intros. subst. destruct_one_match. 2: reflexivity.
+  eapply defuel_loop_inv'; eassumption.
+Qed.
+
+Section RegAlloc.
+
+  Context {width} {BW: Bitwidth width} {word: word.word width} {word_ok: word.ok word}.
+  Context {mem: map.map word byte}.
+  Context {srcLocals: map.map srcvar word}.
+  Context {impLocals: map.map impvar word}.
+  Context {srcLocalsOk: map.ok srcLocals}.
+  Context {impLocalsOk: map.ok impLocals}.
+  Context {srcEnv: map.map String.string (list srcvar * list srcvar * stmt)}.
+  Context {impEnv: map.map String.string (list impvar * list impvar * stmt')}.
+  Context {ext_spec: Semantics.ExtSpec}.
+
+  Definition states_compat(st: srcLocals)(corresp: list (srcvar * impvar))(st': impLocals) :=
+    forall (x: srcvar) (x': impvar),
+      assert_in x x' corresp = Some tt ->
+      forall w,
+        map.get st x = Some w ->
+        map.get st' x' = Some w.
+
+  Definition precond(corresp: list (srcvar * impvar))(s: stmt)(s': stmt'): list (srcvar * impvar) :=
+    match s, s' with
+    | SLoop s1 c s2, SLoop s1' c' s2' => loop_inv corresp s1 s2 s1' s2'
+    | _, _ => corresp
     end.
 
+  Lemma states_compat_eval_bcond: forall lH lL c c' b corresp,
+      check_bcond corresp c c' = Some tt ->
+      eval_bcond lH c = Some b ->
+      states_compat lH corresp lL ->
+      eval_bcond lL c' = Some b.
+  Proof.
+    intros. rename H1 into C. unfold states_compat in C.
+    destruct c; cbn in *; simp; cbn.
+  Admitted.
+  (*
+    {
+      erewrite C. 1: eassumption.
+
+      erewrite ?C by eauto using map.reverse_get_to_get; reflexivity.
+  Qed.
+  *)
+
+  Lemma states_compat_eval_bcond_None: forall lH lL c c' corresp,
+      check_bcond corresp c c' = Some tt ->
+      eval_bcond lH c <> None ->
+      states_compat lH corresp lL ->
+      eval_bcond lL c' <> None.
+  Proof.
+    intros. destr (eval_bcond lH c). 2: congruence.
+    erewrite states_compat_eval_bcond; eassumption.
+  Qed.
+
+  Lemma states_compat_eval_bcond_bw: forall lH lL c c' b corresp,
+      check_bcond corresp c c' = Some tt ->
+      eval_bcond lL c' = Some b ->
+      states_compat lH corresp lL ->
+      eval_bcond lH c <> None ->
+      eval_bcond lH c = Some b.
+  Proof.
+    intros. destr (eval_bcond lH c). 2: congruence.
+    symmetry. rewrite <- H0. eapply states_compat_eval_bcond; eassumption.
+  Qed.
+
+  Lemma states_compat_extends: forall lH m1 m2 lL,
+      extends m1 m2 ->
+      states_compat lH m1 lL ->
+      states_compat lH m2 lL.
+  Proof.
+    unfold states_compat, extends. intros. eauto.
+  Qed.
+
+  Lemma states_compat_precond: forall lH corresp lL s s',
+      states_compat lH corresp lL ->
+      states_compat lH (precond corresp s s') lL.
+  Proof.
+    intros.
+    destruct s; cbn; try assumption.
+    destruct s'; cbn; try assumption.
+    eapply states_compat_extends. 2: eassumption.
+    eapply extends_loop_inv.
+  Qed.
+  Hint Resolve states_compat_precond : states_compat.
+
+  Lemma states_compat_get: forall corresp lL lH y y' v,
+      states_compat lH corresp lL ->
+      assert_in y y' corresp = Some tt ->
+      map.get lH y = Some v ->
+      map.get lL y' = Some v.
+  Proof. unfold states_compat. eauto. Qed.
+
+  Lemma states_compat_put: forall lH corresp lL x x' v,
+      states_compat lH corresp lL ->
+      states_compat (map.put lH x v) (assignment corresp x x') (map.put lL x' v).
+  Proof.
+    intros. unfold states_compat in *. intros k k'. intros.
+    rewrite map.get_put_dec. rewrite map.get_put_dec in H1.
+    unfold assert_in, assignment in H0. simp. simpl in E.
+    rewrite String.eqb_sym, Z.eqb_sym in E.
+    destr (Z.eqb x' k').
+    - subst k'.
+      destr (String.eqb x k).
+      + assumption.
+      + simpl in E. eapply find_some in E. destruct E as [E F].
+        destruct p. eapply Bool.andb_true_iff in F. destruct F as [F1 F2].
+        eapply String.eqb_eq in F1. subst s.
+        eapply Z.eqb_eq in F2. subst z.
+        exfalso. eapply not_In_remove_by_snd in E. exact E.
+    - rewrite Bool.andb_false_r in E.
+      eapply find_some in E. destruct E as [E F].
+      destruct p. eapply Bool.andb_true_iff in F. destruct F as [F1 F2].
+      eapply String.eqb_eq in F1. subst s.
+      eapply Z.eqb_eq in F2. subst z.
+      eapply In_remove_by_snd in E. apply proj1 in E.
+      eapply In_remove_by_fst in E. destruct E.
+      destr (String.eqb x k).
+      + exfalso. congruence.
+      + eapply H. 2: eassumption. unfold assert_in.
+        destruct_one_match. 1: reflexivity.
+        eapply find_none in E1. 2: eassumption.
+        simpl in E1. rewrite String.eqb_refl, Z.eqb_refl in E1. discriminate.
+  Qed.
+
+  Hint Constructors exec.exec : checker_hints.
+  Hint Resolve states_compat_get : checker_hints.
+  Hint Resolve states_compat_put : checker_hints.
+
+  Lemma checker_correct: forall (e: srcEnv) (e': impEnv) s t m lH mc post,
+      (forall f argnames retnames body,
+          map.get e f = Some (argnames, retnames, body) ->
+          exists args binds body' corresp,
+            map.get e' f = Some (map snd args, map snd binds, body') /\
+            argnames = map fst args /\
+            retnames = map fst binds /\
+            check args body body' = Some corresp /\
+            extends corresp binds (* TODO maybe just invoke check_fun instead? *)) ->
+      exec e s t m lH mc post ->
+      forall lL corresp corresp' s',
+      check corresp s s' = Some corresp' ->
+      states_compat lH (precond corresp s s') lL ->
+      exec e' s' t m lL mc (fun t' m' lL' mc' =>
+        exists lH', states_compat lH' corresp' lL' /\ post t' m' lH' mc').
+  Proof.
+    induction 2; intros;
+      match goal with
+      | H: check _ _ _ = Some _ |- _ => pose proof H as C; move C at top; cbn [check] in H
+      end;
+      simp;
+      repeat match goal with
+             | u: unit |- _ => destruct u
+             end.
+
+    - (* Case exec.interact *)
+      case TODO_sam.
+    - (* Case exec.call *)
+      case TODO_sam.
+    - (* Case exec.load *)
+      case TODO_sam.
+    - (* Case exec.store *)
+      case TODO_sam.
+    - (* Case exec.inlinetable *)
+      case TODO_sam.
+    - (* Case exec.stackalloc *)
+      case TODO_sam.
+    - (* Case exec.lit *)
+      case TODO_sam.
+    - (* Case exec.op *)
+      case TODO_sam.
+    - (* Case exec.set *)
+      eauto 10 with checker_hints.
+    - (* Case exec.if_true *)
+      eapply exec.if_true. 1: eauto using states_compat_eval_bcond.
+      eapply exec.weaken.
+      + eapply IHexec. 1: eassumption.
+        cbn [precond] in *. eapply states_compat_precond. eassumption.
+      + cbv beta. intros. simp. eexists. split. 2: eassumption.
+        eapply states_compat_extends. 2: eassumption. eapply extends_intersect_l.
+    - (* Case exec.if_false *)
+      eapply exec.if_false. 1: eauto using states_compat_eval_bcond.
+      eapply exec.weaken.
+      + eapply IHexec. 1: eassumption.
+        cbn [precond] in *. eapply states_compat_precond. eassumption.
+      + cbv beta. intros. simp. eexists. split. 2: eassumption.
+        eapply states_compat_extends. 2: eassumption. eapply extends_intersect_r.
+    - (* Case exec.loop *)
+      rename H4 into IH2, IHexec into IH1, H6 into IH12.
+      match goal with
+      | H: states_compat _ _ _ |- _ => rename H into SC
+      end.
+      cbn [precond] in SC.
+      pose proof SC as SC0.
+      unfold loop_inv in SC.
+      rewrite E in SC.
+      eapply exec.loop.
+      + eapply IH1. 1: eassumption. eapply states_compat_precond. exact SC.
+      + cbv beta. intros. simp. eauto using states_compat_eval_bcond_None.
+      + cbv beta. intros. simp. eexists. split. 2: eauto using states_compat_eval_bcond_bw. assumption.
+      + cbv beta. intros. simp. eapply IH2; eauto using states_compat_eval_bcond_bw.
+        eapply states_compat_precond. assumption.
+      + cbv beta. intros. simp. eapply IH12. 1: eassumption. 1: eassumption.
+        rename l0 into inv. cbn [precond].
+        eapply states_compat_extends. 2: eassumption.
+        pose proof defuel_loop_inv as P.
+        specialize P with (2 := E0).
+        specialize P with (2 := E2).
+        specialize (P corresp).
+        unfold loop_inv in P|-*.
+        rewrite E in P. rewrite E.
+        specialize (P eq_refl).
+        rewrite P.
+        eapply extends_intersect_r.
+    - (* Case exec.seq *)
+      rename H2 into IH2, IHexec into IH1.
+      eapply exec.seq.
+      + eapply IH1. 1: eassumption.
+        cbn [precond] in *. eapply states_compat_precond. assumption.
+      + cbv beta. intros. simp.
+        eapply IH2. 1: eassumption. 1: eassumption.
+        eapply states_compat_precond. assumption.
+    - (* Case exec.skip *)
+      eapply exec.skip. eauto.
+  Qed.
+
 End RegAlloc.
+
+(* Print Assumptions checker_correct. *)
